src/rewriting.ml
@@ -53,7 +53,7 @@ let elim_double_negation f =
     | LessEq (t1, t2) -> LessEq (t1, t2)
     | Pred p -> Pred p
     | Let (p,f1,f2) -> Let (p,elim f1, elim f2)
-    | LetPrev (p,f1,f2) -> LetPrev (p,elim f1, elim f2)
+    | LetPast (p,f1,f2) -> LetPast (p,elim f1, elim f2)
 
     | Neg (Neg f) -> elim f
 
@@ -103,7 +103,7 @@ let simplify_terms f =
       let new_tlist = List.map st tlist in
       Pred (Predicate.make_predicate (name, new_tlist))
     | Let (p,f1,f2) -> Let (p, s f1, s f2)
-    | LetPrev (p,f1,f2) -> LetPrev (p, s f1, s f2)
+    | LetPast (p,f1,f2) -> LetPast (p, s f1, s f2)
     | Neg f -> Neg (s f)
     | And (f1, f2) -> And (s f1, s f2)
     | Or (f1, f2) -> Or (s f1, s f2)
@@ -145,7 +145,7 @@ let rec elim_syntactic_sugar g =
     | Equal _ | Less _ | LessEq _ | Pred _ -> f
 
     | Let (p,f1,f2) -> Let (p, elim f1, elim f2)
-    | LetPrev (p,f1,f2) -> LetPrev (p, elim f1, elim f2)
+    | LetPast (p,f1,f2) -> LetPast (p, elim f1, elim f2)
     | Neg f -> Neg (elim f)
     | And (f1, f2) -> And (elim f1, elim f2)
     | Or (f1, f2) -> Or (elim f1, elim f2)
@@ -210,7 +210,7 @@ let push_negation g =
 
     | Neg f -> Neg (push f)
     | Let (p,f1,f2) -> Let (p,f1, push f2)
-    | LetPrev (p,f1,f2) -> LetPrev (p,f1, push f2)
+    | LetPast (p,f1,f2) -> LetPast (p,f1, push f2)
     | Equal _ | Less _ | LessEq _ | Pred _ -> f
     | And (f1, f2) -> And (push f1, push f2)
     | Or (f1, f2) -> Or (push f1, push f2)
@@ -354,7 +354,7 @@ let rec is_monitorable f =
     then (is_mon1, r1)
     else is_monitorable f2
 
-  | LetPrev (p,f1,f2) ->
+  | LetPast (p,f1,f2) ->
     let (is_mon1, r1) = is_monitorable f1 in
     if not is_mon1
     then (is_mon1, r1)
@@ -565,8 +565,10 @@ let rec rr = function
     (rr2, b1 && b2)
   | Frex (_,r) -> rr_re true r 
   | Prex (_,r) -> rr_re false r 
+  (* TODO: We should also check the first subformula of Let and LetPast, and
+     set the boolean result accordingly. *)
   | Let (_,_,f) -> rr f
-  | LetPrev (_,_,f) -> rr f
+  | LetPast (_,_,f) -> rr f
   | _ -> failwith "[Rewriting.rr] internal error"
   and rr_re future = function 
   | Wild -> ([],true)
@@ -798,7 +800,7 @@ function
   | Equiv (f1, f2)
   | Let (_,f1,f2)
     -> (check_intervals f1) && (check_intervals f2)
-  | LetPrev (_,f1,f2)
+  | LetPast (_,f1,f2)
     -> (check_intervals f1) && (check_intervals f2)
 
   | Eventually (intv, f)
@@ -860,7 +862,7 @@ function
   | Since (_, f1, f2)
   | Let (_,f1,f2)
     -> (check_bounds f1) && (check_bounds f2)
-  | LetPrev (_,f1,f2)
+  | LetPast (_,f1,f2)
     -> (check_bounds f1) && (check_bounds f2)
 
   | Eventually (intv, f)
@@ -906,7 +908,7 @@ let rec is_future = function
   | Since (_, f1, f2)
   | Let (_,f1,f2)
     -> (is_future f1) || (is_future f2)
-  | LetPrev (_,f1,f2)
+  | LetPast (_,f1,f2)
     -> (is_future f1) || (is_future f2)
 
   | Next (_, _)
@@ -949,27 +951,27 @@ let rec check_let = function
     else ();
     check_let f1 && check_let f2
 
-  | LetPrev (p,f1,f2) -> 
+  | LetPast (p,f1,f2) -> 
     let (n,a,ts) = get_info p in
     let check_params = List.for_all (fun t -> match t with Var _ -> true | _ -> false) ts in
     if not check_params
     then 
       let string_of_terms = List.fold_left (fun s v -> s ^ " " ^ string_of_term v) "" in
-      let str = Printf.sprintf "[Rewriting.check_let] LETPREV %s's parameters %s must be variables" n (string_of_terms ts) 
+      let str = Printf.sprintf "[Rewriting.check_let] LETPAST %s's parameters %s must be variables" n (string_of_terms ts) 
       in failwith str
     else ();
     let prms = List.flatten (List.map tvars ts) in 
     let fv1 = free_vars f1 in
     if (List.length fv1) != a
     then 
-      let str = Printf.sprintf "[Rewriting.check_let] LETPREV %s's arity %n must match the number \
+      let str = Printf.sprintf "[Rewriting.check_let] LETPAST %s's arity %n must match the number \
       of free variables of %s " n a (string_of_formula "" f1)
       in failwith str
     else ();
     if not (Misc.subset fv1 prms && Misc.subset prms fv1)
     then 
       let string_of_vars = List.fold_left (fun s v -> s ^ " " ^ string_of_var v) "" in
-      let str = Printf.sprintf "[Rewriting.check_let] LETPREV %s's parameters %s do not coincide with \
+      let str = Printf.sprintf "[Rewriting.check_let] LetPast %s's parameters %s do not coincide with \
       free variables %s of %s" n (string_of_vars prms) (string_of_vars fv1) (string_of_formula "" f1)
       in failwith str
     else ();
@@ -1031,7 +1033,7 @@ let expand_let f =
   | Let (p, f1, f2) ->
     let (n,a,ts) = get_info p in
     expand_let_rec (((n, a), (ts, f1))::m) f2
-  | LetPrev (p, f1, f2) -> failwith "Cannot unfold LETPREV"
+  | LetPast (p, f1, f2) -> failwith "Cannot unfold LETPAST"
 
   | Neg f -> Neg (expand_let_rec m f)
   | Exists (v, f) -> Exists (v,expand_let_rec m f)
@@ -1321,7 +1323,7 @@ let rec type_check_formula (sch, vars) f =
     let new_delta = List.filter (fun (p,_) -> not ((n,a)=p)) s2 in
     (shadowed_pred@new_delta, v2, Let(p,f1,f2))
 
-  | LetPrev (p, f1, f2) -> 
+  | LetPast (p, f1, f2) -> 
     let (n,a,ts) = get_info p in
     let new_vars = List.map (fun v -> match v with (Var t) -> t | _ -> failwith "Internal error") ts in (* We allow only variables here with check_let *)
     let new_typed_vars = List.fold_left (fun vrs vr -> (vr,new_type_symbol TAny vrs)::vrs) [] new_vars in
@@ -1334,7 +1336,7 @@ let rec type_check_formula (sch, vars) f =
     let delta = ((n,a),new_sig)::rest in
     let (s2, v2, f2) = type_check_formula (delta,vars) f2 in
     let new_delta = List.filter (fun (p,_) -> not ((n,a)=p)) s2 in
-    (shadowed_pred@new_delta, v2, LetPrev(p,f1,f2))
+    (shadowed_pred@new_delta, v2, LetPast(p,f1,f2))
 
   | Neg f -> let (s,v,f) = type_check_formula (sch, vars) f in (s,v, Neg f)
   | Prev (intv,f) -> let (s,v,f) = type_check_formula (sch, vars) f in (s,v, Prev (intv,f))
